theories/simplang/primitive_laws.v
@@ -17,14 +17,14 @@ the basic laws of the program logic, assuming that [sheapInv] allows
 them. *)
 
 Class sheapGS (Σ: gFunctors) := SHeapGS {
-  sheapG_gen_progG :> gen_sim_progGS string ectx ectx Σ;
-  sheapG_heapG :> heapG Σ;
+  sheapG_gen_progG :> gen_sim_progGS string ectx ectx Σ | 1;
+  sheapG_heapG :> heapG Σ | 1;
   sheapG_heap_target : heap_names;
   sheapG_heap_source : heap_names;
 }.
 Class sheapGpreS (Σ: gFunctors) := SHeapGpreS {
-  sbij_pre_heapG :> heapG Σ;
-  sbij_pre_progG :> gen_progGpreS Σ string ectx;
+  sbij_pre_heapG :> heapG Σ | 10;
+  sbij_pre_progG :> gen_progGpreS Σ string ectx | 10;
 }.
 Definition sheapΣ := #[heapΣ; gen_progΣ string ectx].
 Global Instance subG_sheapΣ Σ :
@@ -40,7 +40,7 @@ Class sheapInv (Σ : gFunctors) := SHeapRel {
   sheap_inv : prog → state → list expr → iProp Σ;
   sheap_inv_pure_prim_step P_s σ_s e_s T π e_s':
     T !! π = Some e_s →
-    (∀ σ_s, prim_step P_s e_s σ_s e_s' σ_s []) →
+    (∀ σ_s', σ_s'.(globals) = σ_s.(globals) → prim_step P_s e_s σ_s' e_s' σ_s' []) →
     sheap_inv P_s σ_s T -∗
     sheap_inv P_s σ_s (<[π:=e_s']>T);
   sheap_ext_rel : thread_id → val → val → iProp Σ;
@@ -82,10 +82,11 @@ Class sheapInvSupportsAlloc `{!sheapInv Σ} := {
     sheap_inv P_s σ_s T_s -∗
     sheap_inv P_s
          {| heap :=
-             heap_array (Loc (fresh_block (heap σ_s) (used_blocks σ_s)) 0)
+             heap_array (dyn_loc (fresh (used_dyn_blocks σ_s)))
                (replicate (Z.to_nat n) v) ∪ heap σ_s;
-           used_blocks := {[fresh_block (heap σ_s) (used_blocks σ_s)]} ∪ used_blocks σ_s
-         |} (<[π:=fill K_s #(Loc (fresh_block (heap σ_s) (used_blocks σ_s)) 0)]> T_s);
+           used_dyn_blocks := {[fresh (used_dyn_blocks σ_s)]} ∪ used_dyn_blocks σ_s;
+           globals := globals σ_s
+         |} (<[π:=fill K_s #(dyn_loc (fresh (used_dyn_blocks σ_s)))]> T_s);
 }.
 Class sheapInvSupportsFree `{!sheapInv Σ} := {
   sheap_inv_free P_s σ_s T_s (n : Z) (l : loc) K_s π:
@@ -195,23 +196,31 @@ Notation "† l '…s' n" := (heap_freeable sheapG_heap_source l 1 (Some n))
 Notation "† l '…s' -" := (heap_freeable sheapG_heap_source l 1 None)
   (at level 20, format "† l …s  -") : bi_scope.
 
-Lemma sheap_init `{!sheapGpreS Σ} P_t h_t P_s h_s T_s :
+(** Global *)
+Notation target_globals := (heap_globals sheapG_heap_target).
+Notation target_global := (heap_global sheapG_heap_target).
+Notation source_globals := (heap_globals sheapG_heap_source).
+Notation source_global := (heap_global sheapG_heap_source).
+
+Lemma sheap_init `{!sheapGpreS Σ} P_t g_t P_s g_s T_s :
   ⊢@{iPropI Σ} |==> ∃ `(!sheapGS Σ), ∀ `(!sheapInv Σ),
-    (sheap_inv P_s (state_init h_s) T_s -∗
-      state_interp P_t (state_init h_t) P_s (state_init h_s) T_s) ∗
-    ([∗ map] f ↦ K ∈ P_t, f @t K) ∗ ([∗ map] l ↦ v ∈ h_t, l ↦t v) ∗
-    ([∗ map] f ↦ K ∈ P_s, f @s K) ∗ ([∗ map] l ↦ v ∈ h_s, l ↦s v) ∗
+    (sheap_inv P_s (state_init g_s) T_s -∗
+      state_interp P_t (state_init g_t) P_s (state_init g_s) T_s) ∗
+    ([∗ map] f ↦ K ∈ P_t, f @t K) ∗ ([∗ map] n ↦ v ∈ g_t, global_loc n ↦t v ∗ †global_loc n …t 1) ∗
+    ([∗ map] f ↦ K ∈ P_s, f @s K) ∗ ([∗ map] n ↦ v ∈ g_s, global_loc n ↦s v ∗ †global_loc n …s 1) ∗
+    source_globals (dom _ g_s) ∗ target_globals (dom _ g_t) ∗
     progs_are P_t P_s.
 Proof.
-  iMod (heap_init h_t) as (γheap_tgt) "[Hheap_tgt Hptsto_tgt]".
-  iMod (heap_init h_s) as (γheap_src) "[Hheap_src Hptsto_src]".
+  iMod (heap_init g_t) as (γheap_tgt) "(Hheap_tgt & #Hg_tgt & Hptsto_tgt)".
+  iMod (heap_init g_s) as (γheap_src) "(Hheap_src & #Hg_src & Hptsto_src)".
   iMod (gen_sim_prog_init P_t P_s) as (?) "[#Hprog_tgt #Hprog_src]".
   iExists (SHeapGS _ _ _ γheap_tgt γheap_src). iIntros "!> %".
   iFrame. iSplitL; last iSplit; last iSplit.
   - iIntros "?". rewrite /state_interp /=. iFrame "∗#".
   - by iApply has_prog_all_funs.
   - by iApply has_prog_all_funs.
-  - rewrite /progs_are /=. iIntros "!#" (P_t' P_s' σ_t' σ_s' T_s') "(#Hprog_tgt2 & #Hprog_src2 & _)".
+  - iFrame "Hg_tgt Hg_src".
+    rewrite /progs_are /=. iIntros "!#" (P_t' P_s' σ_t' σ_s' T_s') "(#Hprog_tgt2 & #Hprog_src2 & _)".
     iDestruct (has_prog_agree with "Hprog_tgt Hprog_tgt2") as %->.
     iDestruct (has_prog_agree with "Hprog_src Hprog_src2") as %->.
     done.
@@ -236,45 +245,73 @@ Lemma has_fun_source_agree f K_s1 K_s2 : f @s K_s1 -∗ f @s K_s2 -∗ ⌜K_s1 =
 Proof. apply has_fun_agree. Qed.
 
 
+(** operational lemmas for global variables *)
+Lemma target_red_global n Ψ :
+  target_global n -∗
+  target_red #(global_loc n) Ψ -∗
+  target_red (GlobalVar n) Ψ.
+Proof.
+  iIntros "Hg Hred". iApply target_red_lift_head_step.
+  iIntros (?????) "(HP_t & HP_s & Hσ_t & Hσ_s & ?) !>".
+  iDestruct (heap_global_in_ctx with "Hσ_t Hg") as %?.
+  iSplitR; first by eauto with head_step.
+  iIntros (e_t' efs σ_t') "%"; inv_head_step.
+  iModIntro. by iFrame.
+Qed.
+
+Lemma source_red_global n Ψ π :
+  (source_global n -∗ source_red #(global_loc n) π Ψ) -∗
+  source_red (GlobalVar n) π Ψ.
+Proof.
+  iIntros "Hred". iApply source_red_lift_head_step.
+  iIntros (??????) "[(HP_t & HP_s & Hσ_t & Hσ_s & ?) [% %Hsafe]] !>".
+  have ?:= pool_safe_irred _ _ _ _ _ _ _ Hsafe ltac:(done) ltac:(done).
+  iDestruct (heap_global_intro_ctx with "Hσ_s") as "#Hg"; [done|].
+  iExists _, _. iSplit. { simpl. eauto with head_step. }
+  iModIntro. iDestruct ("Hred" with "[//]") as "$". iFrame.
+  iApply sheap_inv_pure_prim_step; [done| |done] => ??.
+  apply: fill_prim_step. apply: head_prim_step. econstructor. set_solver.
+Qed.
+
 (** operational heap lemmas *)
 
 Lemma target_red_allocN n v Ψ:
   (0 < n)%Z →
-  (∀ l, l ↦t∗ (replicate (Z.to_nat n) v) -∗
+  (∀ l, ⌜block_is_dyn l.(loc_block)⌝ -∗ l ↦t∗ (replicate (Z.to_nat n) v) -∗
     † l …t (Z.to_nat n) -∗ target_red (of_val #l) Ψ) -∗
   target_red (AllocN (Val $ LitV $ LitInt $ n) (Val v)) Ψ.
 Proof.
   iIntros (Hn) "Hloc". iApply target_red_lift_head_step.
   iIntros (P_s σ_s P_t σ_t T_s) "(HP_t & HP_s & Hσ_t & Hσ_s & Hinv)". iModIntro.
+  iDestruct (heap_ctx_wf with "Hσ_t") as %?.
   iSplitR. { eauto using alloc_fresh with head_step. }
   iIntros (e_t' efs_t σ_t') "%"; inv_head_step.
-  set (l := Loc b 0).
-  iMod (heap_alloc _ _ l with "Hσ_t") as "($&Hn&Hm)"; [done..|].
+  iMod (heap_alloc _ _ b with "Hσ_t") as "($&Hn&Hm)"; [done..|].
   iModIntro. iFrame. iSplitR; first done.
-  by iApply ("Hloc" with "Hm Hn").
+  by iApply ("Hloc" with "[] Hm Hn").
 Qed.
 
 Lemma source_red_allocN π n v Ψ `{!sheapInvSupportsAlloc}:
   (0 < n)%Z →
-  (∀ l, l ↦s∗ (replicate (Z.to_nat n) v) -∗
+  (∀ l, ⌜block_is_dyn l.(loc_block)⌝ -∗ l ↦s∗ (replicate (Z.to_nat n) v) -∗
   † l …s Z.to_nat n -∗ source_red (of_val #l) π Ψ) -∗
   source_red (AllocN (Val $ LitV $ LitInt $ n) (Val v)) π Ψ.
 Proof.
   iIntros (Hn) "Hloc". iApply source_red_lift_head_step.
   iIntros (P_s σ_s P_t σ_t T_s K_s) "[(HP_t & HP_s & Hσ_t & Hσ_s & Hinv) [% %]]".
-  iDestruct (heap_ctx_wf with "Hσ_s") as %?.
+  iDestruct (heap_ctx_wf with "Hσ_s") as %Hwf.
   iExists _, _. iSplitR. { simpl. eauto using alloc_fresh with lia head_step. }
   simpl.
-  iMod (heap_alloc _ _ (Loc (fresh_block (heap σ_s) (used_blocks σ_s)) 0) with "Hσ_s") as "($&Hn&Hm)"; [done|done| | |].
-  { apply is_fresh_block_blocks. }
-  { move => ?. apply is_fresh_block. }
+  iMod (heap_alloc _ _ (fresh (used_dyn_blocks σ_s)) with "Hσ_s") as "($&Hn&Hm)"; [done| | |].
+  { apply is_fresh. }
+  { move => ?. apply eq_None_not_Some => -[? /Hwf]. apply is_fresh. }
   iModIntro. iFrame.
   iSplitL "Hinv". { by iApply sheap_inv_alloc. }
-  by iApply ("Hloc" with "Hm Hn").
+  by iApply ("Hloc" with "[] Hm Hn").
 Qed.
 
 Lemma target_red_alloc v Ψ:
-  (∀ l, l ↦t v -∗ † l …t 1 -∗ target_red (of_val #l) Ψ) -∗
+  (∀ l, ⌜block_is_dyn l.(loc_block)⌝ -∗ l ↦t v -∗ † l …t 1 -∗ target_red (of_val #l) Ψ) -∗
   target_red (Alloc (Val v)) Ψ.
 Proof.
   iIntros "Ht". iApply (target_red_allocN); first lia.
@@ -283,7 +320,7 @@ Proof.
 Qed.
 
 Lemma source_red_alloc π v Ψ `{!sheapInvSupportsAlloc} :
-  (∀ l, l ↦s v -∗ † l …s 1 -∗ source_red (of_val #l) π Ψ) -∗
+  (∀ l, ⌜block_is_dyn l.(loc_block)⌝ -∗ l ↦s v -∗ † l …s 1 -∗ source_red (of_val #l) π Ψ) -∗
   source_red (Alloc (Val v)) π Ψ.
 Proof.
   iIntros "Ht". iApply (source_red_allocN); first lia.
@@ -332,8 +369,7 @@ Proof.
   rewrite heap_mapsto_vec_to_st.
   iMod (heap_free with "Hσ_s Hl Hn") as (??) "[? ?]"; [ done | ].
   iExists (Val #()), (state_upd_heap (free_mem l _) σ_s).
-  iSplitR; first eauto with lia head_step.
-  { iPureIntro. econstructor; eauto with lia. }
+  iSplitR. { iPureIntro. econstructor; eauto with lia. }
   iModIntro. iModIntro. iFrame.
   iSplitL "Hinv". { by iApply sheap_inv_free. }
     by iApply "Hsim".
@@ -522,7 +558,7 @@ Proof.
   iDestruct (has_prog_has_fun_agree with "HP_s Hf") as %?.
   iExists _, _. iSplit. { simpl. eauto with head_step. }
   iModIntro. iFrame.
-  iApply sheap_inv_pure_prim_step; [done| |done] => ?.
+  iApply sheap_inv_pure_prim_step; [done| |done] => ??.
   apply: fill_prim_step. apply: head_prim_step. by constructor.
 Qed.
 
@@ -579,7 +615,7 @@ Proof.
   iModIntro. iExists e_s', σ_s'. inv_head_step. iFrame. iSplit;[done|].
   iSplitR; first by eauto with head_step.
   iSplitL "Hsi". {
-    iApply sheap_inv_pure_prim_step; [done| |done] => ?.
+    iApply sheap_inv_pure_prim_step; [done| |done] => ??.
     apply: fill_prim_step. apply: head_prim_step. by constructor.
   }
   iApply "Hstep". iFrame.
@@ -605,7 +641,7 @@ Proof.
   iDestruct (has_prog_has_fun_agree with "HP_s Hrec") as %?.
   iFrame. iSplitR; [done|].
   iSplitR; [by eauto with head_step|].
-  iApply sheap_inv_pure_prim_step; [done| |done] => ?.
+  iApply sheap_inv_pure_prim_step; [done| |done] => ??.
   apply: fill_prim_step. apply: head_prim_step. by constructor.
 Qed.
 
@@ -630,7 +666,7 @@ Proof.
   { eauto with head_step. }
   iExists e_s', σ_s'. inv_head_step. iFrame. iSplitR; [done|].
   iSplitR; [by eauto with head_step|].
-  iApply sheap_inv_pure_prim_step; [done| |done] => ?.
+  iApply sheap_inv_pure_prim_step; [done| |done] => ??.
   apply: fill_prim_step. apply: head_prim_step. by constructor.
 Qed.
 
@@ -660,7 +696,7 @@ Proof.
   iExists e_s', σ_s'. inv_head_step. iFrame.
   iSplitR; [done|].
   iSplitR; [by eauto with head_step|].
-  iApply sheap_inv_pure_prim_step; [done| |done] => ?.
+  iApply sheap_inv_pure_prim_step; [done| |done] => ??.
   apply: fill_prim_step. apply: head_prim_step. by constructor.
 Qed.
 End lifting.
