theories/simplang/gen_global_rel.v
@@ -1,0 +1,53 @@
+From simuliris.simulation Require Import slsls lifting.
+From simuliris.simplang Require Import proofmode tactics.
+From simuliris.simplang Require Import parallel_subst primitive_laws gen_log_rel gen_val_rel.
+
+(** * Generic relation for global variables
+
+This file defines [gen_global_rel] that relates the global variables
+of source and target. It is used to prove the reflexivity of
+[GlobalVar x]. *)
+
+Section gen_global_rel.
+  Context `{!sheapGS Σ} `{!sheapInv Σ}.
+  Context (loc_rel : loc → loc → iProp Σ).
+  Context (thread_own : thread_id → iProp Σ).
+  Let log_rel := (gen_log_rel loc_rel thread_own).
+
+  Definition gen_global_rel (g_t g_s : gset string) : iProp Σ :=
+    ⌜g_s ⊆ g_t⌝ ∗ target_globals g_t ∗ source_globals g_s ∗
+     [∗ set] g∈g_s, loc_rel (global_loc g) (global_loc g).
+
+  Global Instance gen_global_rel_persistent g_t g_s `{!∀ l_t l_s, Persistent (loc_rel l_t l_s)}:
+    Persistent (gen_global_rel g_t g_s).
+  Proof. apply _. Qed.
+
+  Definition gen_global_rel_law : Prop :=
+    (∀ Φ, (∀ g_t g_s, gen_global_rel g_t g_s -∗ Φ) -∗ update_si Φ).
+
+  Lemma source_red_global' n Ψ π :
+    gen_global_rel_law →
+    (target_global n -∗ source_global n -∗ loc_rel (global_loc n) (global_loc n) -∗
+                   source_red #(global_loc n) π Ψ) -∗
+    source_red (GlobalVar n) π Ψ.
+  Proof.
+    iIntros (Hrel) "Hred".
+    iApply source_red_update_si. iApply Hrel. iIntros (g_t g_s) "(%Hsub&Hgs_t&Hgs_s&Hrel)".
+    iApply source_red_global. iIntros "#Hg_s".
+    iDestruct (heap_global_in with "Hgs_s Hg_s") as %Hin. move: (Hin) => /Hsub?.
+    iDestruct (heap_global_intro with "Hgs_t") as "#Hg_t"; [done|].
+    iApply "Hred"; [done..|].
+    by iApply (big_sepS_elem_of with "Hrel").
+  Qed.
+
+  Lemma log_rel_global_var x :
+    gen_global_rel_law →
+    ⊢ log_rel (GlobalVar x) (GlobalVar x).
+  Proof.
+    iIntros (Hrel ? xs) "!# Hs Ht"; simpl.
+    iApply source_red_sim_expr. iApply source_red_global'; [done|]. iIntros "#Hg_t #Hg_s Hv".
+    iApply source_red_base. iModIntro.
+    iApply target_red_sim_expr. iApply (target_red_global with "Hg_t"). iApply target_red_base. iModIntro.
+    iApply sim_expr_base. iApply lift_post_val. iFrame.
+  Qed.
+End gen_global_rel.
