theories/simplang/na_inv/adequacy.v
@@ -24,25 +24,30 @@ Global Instance subG_naΣ Σ :
   subG naΣ Σ → naGpreS Σ.
 Proof. solve_inG. Qed.
 
-Lemma prog_rel_adequacy Σ `{!naGpreS Σ} (p_t p_s : prog) :
+Lemma prog_rel_adequacy Σ `{!naGpreS Σ} (p_t p_s : prog) gs :
   isat (∀ `(naGS Σ),
     ([∗ map] f ↦ K ∈ p_t, f @t K) -∗
     ([∗ map] f ↦ K ∈ p_s, f @s K) -∗
-    prog_rel p_t p_s
+    target_globals (dom (gset string) gs) -∗
+    source_globals (dom (gset string) gs) ==∗
+    ([∗ map] v∈gs, val_rel v v) ∗ prog_rel p_t p_s
   ) →
-  beh_rel p_t p_s.
+  beh_rel gs p_t p_s.
 Proof.
   intros Hprog. apply simplang_adequacy.
   eapply sat_mono, Hprog. clear Hprog.
   iIntros "Hprog_rel %".
-  iMod heapbij_init as (?) "Hbij".
+  iMod (heapbij_init (λ _, alloc_rel_pred [∅])) as (?) "Hbij".
   iMod (ghost_map_alloc) as (γcols) "[Hcols Hcol]".
+  set HΣ := (NaGS Σ _ _ _ γcols).
   iModIntro. iExists na_inv, heapbij.loc_rel.
-  iSpecialize ("Hprog_rel" $! (NaGS Σ _ _ _ γcols)).
-  iFrame "Hprog_rel".
-  iSplitL "Hbij Hcols".
-  - rewrite /sheap_inv. iExists ∅, [∅]. iFrame. iPureIntro. split_and!.
-    + done.
+  iSpecialize ("Hprog_rel" $! HΣ).
+  iIntros "Hp_t Hp_s Hmt #Hgs_t #Hgs_s".
+  iMod ("Hprog_rel" with "[$] [$] [$] [$]") as "[#Hvs $]".
+  iMod (heap_bij_insert_globals with "Hbij Hmt Hvs") as (L') "[Hbij #Hls]"; [done| ].
+  iModIntro. iSplitL "Hbij Hcols".
+  - rewrite /sheap_inv. iExists _, [∅], _. iFrame.
+    repeat iSplit; try done; iPureIntro.
     + apply: na_locs_wf_init.
     + apply: na_locs_in_L_init.
   - rewrite map_seq_cons big_sepM_insert //.
@@ -55,9 +60,11 @@ Theorem log_rel_adequacy Σ `{!naGpreS Σ} e_t e_s :
   (∀ `(naGS Σ), ⊢ log_rel e_t e_s) →
   ctx_rel e_t e_s.
 Proof.
-  intros Hrel C fname x p Hpwf HCwf Hvars.
+  intros Hrel C fname x p gs Hpwf HCwf Hvars Hgs.
   apply (prog_rel_adequacy Σ). eapply isat_intro.
-  iIntros (?) "_ _ !# %f %K_s %π".
+  iIntros (?) "_ _ _ _ !#".
+  iSplit. { iApply big_sepM_intro. iIntros "!>" (???). iApply val_wf_sound. by apply: Hgs. }
+  iIntros "!# %f %K_s %π".
   iDestruct (Hrel _) as "Hrel". clear Hrel.
   destruct (decide (f = fname)) as [->|Hne].
     rewrite !lookup_insert.
